tests/test_notation.v
@@ -1,0 +1,67 @@
+From stdpp Require Import strings.
+From D.Dot Require Import syn exampleInfra hoas.
+From D.Dot Require typingExInfra.
+
+Module TestDB.
+Import DBNotation.
+
+Check {@ TNat ; TNat ; TNat }%ty.
+
+(* Check (TSel (pself (pself p0 1) 2) 3). *)
+(* Check (x0 @ 1 @ 2 ; 3). *)
+
+Check ν {@ val "a" = pv (vnat 0) }.
+
+Check μ {@ type "A" >: TNat <: TTop }.
+Check μ {@ val "a" : TNat }.
+Check μ {@ type "A" >: TNat <: TTop ; val "a" : TNat ; val "b" : TNat }.
+
+Check vobj {@}.
+Check ν {@ }.
+Check ν {@ val "a" = pv (vnat 0) }.
+Check ν {@ val "a" = pv (vnat 0) ; val "b" = pv (vnat 1) }.
+
+Check (p0 @; "A").
+Check (pself (pself p0 "A") "B" @; "C").
+Check (p0 @ "A").
+Check (p0 @ "A" @ "B" @; "C").
+Check (val "symb" : p0 @ "symbols" @; "Symbol")%ty.
+
+Module TestStamped.
+Import typingExInfra.
+Check ν {@ type "A" = (σ1 ; s1) }.
+Check ν {@ val "a" = pv (vnat 0); type "A" = (σ1 ; s1) }.
+Check ν {@ val "a" = pv (vnat 0) ; type "A" = (σ1 ; s1) }.
+End TestStamped.
+End TestDB.
+
+Module hoasTests.
+
+Import hoasNotation hterm_lifting.
+
+Goal hvar_vl = λ n i, var_vl (n + i). done. Abort.
+Goal ∀ n, hvnat n = liftA0 (vnat n). done. Abort.
+Goal hxm = λ i, ren (λ j, j - i). done. Abort.
+
+(** * First test *)
+
+(* ∀ (x : TNat), μ y, x.type ∧ x.type *)
+Definition ex0 := hclose $ hTAll hTNat (λ x, hTMu (λ y, hTAnd (hTSing (hpv x)) (hTSing (hpv y)))).
+Eval cbv in ex0.
+
+Eval cbv -[plus minus] in hTAll.
+Goal hTAll = λ T U i, (TAll (T i) (U (λ x, var_vl (x - S i)) (S i))). done. Abort.
+(* Goal hTAll = λ T U i, (∀ (T i), U (λ x, var_vl (x - S i)) (S i)). done. Abort. *)
+
+Eval cbv in hclose {@ hTNat ; hTNat ; hTNat } %HT.
+
+Definition ex := hclose $ ∀: x : hTNat, hTMu (λ y, hTAnd (hTSing (hpv x)) (hTSing (hpv y))).
+Goal ex = ex0. done. Abort.
+
+Definition ex2 := hclose (λ: f, htv f).
+Eval cbv in ex2.
+Goal ex2 = vabs (tv DBNotation.x0). done. Qed.
+Definition ex3 := hclose (λ:: f x, htapp (htv f) (htv x)).
+Eval cbv in ex3.
+Goal ex3 = tv (vabs (tv (vabs (tapp (tv DBNotation.x1) (tv DBNotation.x0))))). done. Abort.
+End hoasTests.
